dcb/_doc/lean/lakefile.lean
@@ -3,7 +3,8 @@ open Lake DSL
 
 package DCBConflict where
   leanOptions := #[
-    ⟨`autoImplicit, false⟩
+    ⟨`autoImplicit, false⟩,
+    ⟨`linter.unusedVariables, true⟩
   ]
 
 require batteries from git "https://github.com/leanprover-community/batteries" @ "main"
